\documentclass[journal,12pt,twocolumn]{IEEEtran}

\usepackage{setspace}
\usepackage{gensymb}

\singlespacing


\usepackage[cmex10]{amsmath}

\usepackage{amsthm}

\usepackage{mathrsfs}
\usepackage{txfonts}
\usepackage{stfloats}
\usepackage{bm}
\usepackage{cite}
\usepackage{cases}
\usepackage{subfig}

\usepackage{longtable}
\usepackage{multirow}

\usepackage{enumitem}
\usepackage{mathtools}
\usepackage{steinmetz}
\usepackage{tikz}
\usepackage{circuitikz}
\usepackage{verbatim}
\usepackage{tfrupee}
\usepackage[breaklinks=true]{hyperref}
\usepackage{graphicx}
\usepackage{tkz-euclide}
\usepackage{float}

\usetikzlibrary{calc,math}
\usepackage{listings}
    \usepackage{color}                                            %%
    \usepackage{array}                                            %%
    \usepackage{longtable}                                        %%
    \usepackage{calc}                                             %%
    \usepackage{multirow}                                         %%
    \usepackage{hhline}                                           %%
    \usepackage{ifthen}                                           %%
    \usepackage{lscape}     
\usepackage{multicol}
\usepackage{chngcntr}

\DeclareMathOperator*{\Res}{Res}

\renewcommand\thesection{\arabic{section}}
\renewcommand\thesubsection{\thesection.\arabic{subsection}}
\renewcommand\thesubsubsection{\thesubsection.\arabic{subsubsection}}

\renewcommand\thesectiondis{\arabic{section}}
\renewcommand\thesubsectiondis{\thesectiondis.\arabic{subsection}}
\renewcommand\thesubsubsectiondis{\thesubsectiondis.\arabic{subsubsection}}


\hyphenation{op-tical net-works semi-conduc-tor}
\def\inputGnumericTable{}                                 %%

\lstset{
%language=C,
frame=single, 
breaklines=true,
columns=fullflexible
}
\begin{document}
\newtheorem{theorem}{Theorem}[section]
\newtheorem{problem}{Problem}
\newtheorem{proposition}{Proposition}[section]
\newtheorem{lemma}{Lemma}[section]
\newtheorem{corollary}[theorem]{Corollary}
\newtheorem{example}{Example}[section]
\newtheorem{definition}[problem]{Definition}

\newcommand{\BEQA}{\begin{eqnarray}}
\newcommand{\EEQA}{\end{eqnarray}}
\newcommand{\define}{\stackrel{\triangle}{=}}
\bibliographystyle{IEEEtran}
\providecommand{\mbf}{\mathbf}
\providecommand{\pr}[1]{\ensuremath{\Pr\left(#1\right)}}
\providecommand{\qfunc}[1]{\ensuremath{Q\left(#1\right)}}
\providecommand{\sbrak}[1]{\ensuremath{{}\left[#1\right]}}
\providecommand{\lsbrak}[1]{\ensuremath{{}\left[#1\right.}}
\providecommand{\rsbrak}[1]{\ensuremath{{}\left.#1\right]}}
\providecommand{\brak}[1]{\ensuremath{\left(#1\right)}}
\providecommand{\lbrak}[1]{\ensuremath{\left(#1\right.}}
\providecommand{\rbrak}[1]{\ensuremath{\left.#1\right)}}
\providecommand{\cbrak}[1]{\ensuremath{\left\{#1\right\}}}
\providecommand{\lcbrak}[1]{\ensuremath{\left\{#1\right.}}
\providecommand{\rcbrak}[1]{\ensuremath{\left.#1\right\}}}
\theoremstyle{remark}
\newtheorem{rem}{Remark}
\newcommand{\sgn}{\mathop{\mathrm{sgn}}}
\providecommand{\abs}[1]{\vert#1\vert}
\providecommand{\res}[1]{\Res\displaylimits_{#1}} 
\providecommand{\norm}[1]{\lVert#1\rVert}
%\providecommand{\norm}[1]{\lVert#1\rVert}
\providecommand{\mtx}[1]{\mathbf{#1}}
\providecommand{\mean}[1]{E[ #1 ]}
\providecommand{\fourier}{\overset{\mathcal{F}}{ \rightleftharpoons}}
%\providecommand{\hilbert}{\overset{\mathcal{H}}{ \rightleftharpoons}}
\providecommand{\system}{\overset{\mathcal{H}}{ \longleftrightarrow}}
	%\newcommand{\solution}[2]{\textbf{Solution:}{#1}}
\newcommand{\solution}{\noindent \textbf{Solution: }}
\newcommand{\cosec}{\,\text{cosec}\,}
\providecommand{\dec}[2]{\ensuremath{\overset{#1}{\underset{#2}{\gtrless}}}}
\newcommand{\myvec}[1]{\ensuremath{\begin{pmatrix}#1\end{pmatrix}}}
\newcommand{\mydet}[1]{\ensuremath{\begin{vmatrix}#1\end{vmatrix}}}
\numberwithin{equation}{subsection}
\makeatletter
\@addtoreset{figure}{problem}
\makeatother
\let\StandardTheFigure\thefigure
\let\vec\mathbf
\renewcommand{\thefigure}{\theproblem}
\def\putbox#1#2#3{\makebox[0in][l]{\makebox[#1][l]{}\raisebox{\baselineskip}[0in][0in]{\raisebox{#2}[0in][0in]{#3}}}}
     \def\rightbox#1{\makebox[0in][r]{#1}}
     \def\centbox#1{\makebox[0in]{#1}}
     \def\topbox#1{\raisebox{-\baselineskip}[0in][0in]{#1}}
     \def\midbox#1{\raisebox{-0.5\baselineskip}[0in][0in]{#1}}
\vspace{3cm}
\title{ASSIGNMENT 2}
\author{Amulya Tallamraju \\ AI20BTECH11003}
\maketitle
\newpage
\bigskip
\renewcommand{\thefigure}{\theenumi}
\renewcommand{\thetable}{\theenumi}
Download all python codes from 
\begin{lstlisting}
https://github.com/AmulyaTallamraju/EE3900/blob/main/Assignment-2/codes/Assignment-2.py
\end{lstlisting}
%
and latex-tikz codes from 
%
\begin{lstlisting}
https://github.com/AmulyaTallamraju/EE3900/blob/main/Assignment-2/Assignment-2.tex
\end{lstlisting}
%
\section{Matrices 2.4 (iv)}
Let $A=\myvec{2 &4\\3 &2},B=\myvec{1 &3\\-2 &5}.$
Find $AB$
%
\section{Solution}
\begin{align}
AB&=\myvec{(2 \times 1) +(4 \times (-2)) &(2 \times 3) +(4 \times 5)\\(3 \times 1) +(2 \times (-2)) &(3 \times 3) +(2 \times 5)}\\
&=\myvec{-6 &26\\-1 &19}
\end{align}
Let 
\begin{align}
    A&=\myvec{a &b\\c &d}\\
    B&=\myvec{e &f\\g &h}
\end{align}
For the multiplication to be commutative,
\begin{align}
    &\myvec{a &b\\c &d} \cdot \myvec{e &f\\g &h}=\myvec{e &f\\g &h} \cdot \myvec{a &b\\c &d}\\
    \implies& \myvec{ae + bg & af + bh \\
ce + dg & cf + dh}= \myvec{ae + cf & be + df \\
ag + ch & bg + dh} \label{commie}
\end{align}
From \eqref{commie} we get
\begin{align}
  & ae + bg &= ae + cf &\implies bg = cf \\
  & af + bh &= be + df\\
 & ce + dg &= ag + ch\\
 & cf + dh &= bg + dh &\implies cf = bg
\end{align}
Simplifying the above equations further we have
\begin{align}
     bg = cf 
\end{align}
\begin{align}\label{one}
 f (a - d) = b (e - h)
 \end{align}
 \begin{align}\label{two}
 g (a - d) = c (e - h) 
\end{align}
The above equations must hold true for the multiplication of the matrices to be commutative. We have three cases
\begin{enumerate}
    \item $a!=d$ and $e!=h$.
    Dividing \eqref{one} by \eqref{two}
    \begin{align}
        &\frac{f}{g}=\frac{b}{c}\\
        \implies & fc=bg
    \end{align}
    \item $a=d.$
    Substituting in \eqref{one} and \eqref{two}
    \begin{align}
        0=b(e-h)\\
        0=c(e-h)
    \end{align}
    For the above equations to hold true, $e=h$ or $b=c=0$
    \item $e=h.$
    Substituting in \eqref{one} and \eqref{two}
    \begin{align}
        0=f(a-d)\\
        0=g(a-d)
    \end{align}
    For the above equations to hold true, $a=d$ or $f=g=0$
\end{enumerate}
Considering the given $A$ and $B$,
\begin{align}
    b=4,g=-2,c=3,f=3
    bg=-8!=9=cf
\end{align}
Hence, the multiplication of the matrices $A$ and $B$ is not commutative.
This can be verified by observing that
\begin{align}
    BA=\myvec{11 & 10 \\ 11 & 2}
\end{align}
\end{document}
